Prove lookup and domain theorems for mapi

src/patricia/sptreeScript.sml
@@ -585,34 +585,31 @@ val foldi_def = Define`
        foldi f (i + inc) (f i a (foldi f (i + 2 * inc) acc t1)) t2)
 `;
 
-val mapi0_def = Define`
-  (mapi0 f i LN = LN) /\
-  (mapi0 f i (LS a) = LS (f i a)) /\
-  (mapi0 f i (BN t1 t2) =
-   let inc = lrnext i in
-     mk_BN (mapi0 f (i + 2 * inc) t1) (mapi0 f (i + inc) t2)) /\
-  (mapi0 f i (BS t1 a t2) =
-   let inc = lrnext i in
-     mk_BS (mapi0 f (i + 2 * inc) t1) (f i a) (mapi0 f (i + inc) t2))
-`;
-val _ = export_rewrites ["mapi0_def"]
-val mapi_def = Define`mapi f pt = mapi0 f 0 pt`;
+val spt_acc_def = tDefine"spt_acc"`
+  (spt_acc i 0 = i) /\
+  (spt_acc i (SUC k) = spt_acc (i + if EVEN (SUC k) then 2 * lrnext i else lrnext i) (k DIV 2))`
+  (WF_REL_TAC`measure SND`
+   \\ simp[DIV_LT_X]);
 
+val spt_acc_thm = Q.store_thm("spt_acc_thm",
+  `spt_acc i k = if k = 0 then i else spt_acc (i + if EVEN k then 2 * lrnext i else lrnext i) ((k-1) DIV 2)`,
+  rw[spt_acc_def] \\ Cases_on`k` \\ fs[spt_acc_def]);
 
-(*val mapi0_foldi = Q.store_thm(
-  "mapi0_foldi",
-  `mapi0 f i pt = foldi (\n v (i,acc_pt). (insert n (f i v) acc_pt
-*)
+val lemmas = prove(
+    ``(!x. EVEN (2 * x + 2)) /\
+      (!x. ODD (2 * x + 1))``,
+    conj_tac >- (
+      simp[EVEN_EXISTS] >> rw[] >>
+      qexists_tac`SUC x` >> simp[] ) >>
+    simp[ODD_EXISTS,ADD1] >>
+    metis_tac[] )
 
-(*
-        (1,b)                 18
-       /                     /
-  (0,a)       (4,d)        10    42
-       \     /               \  /
-        (2,c)                 26
-             \                  \
-              (6,e)              58
-*)
+val bit_induction = prove(
+  ``!P. P 0 /\ (!n. P n ==> P (2 * n + 1)) /\
+        (!n. P n ==> P (2 * n + 2)) ==>
+        !n. P n``,
+  gen_tac >> strip_tac >> completeInduct_on `n` >> simp[] >>
+  qspec_then `n` strip_assume_tac bit_cases >> simp[]);
 
 val lrnext212 = prove(
   ``(lrnext (2 * m + 1) = 2 * lrnext m) /\
@@ -623,13 +620,6 @@ val lrnext212 = prove(
     `2 * m + 2 = BIT2 m` suffices_by simp[lrnext_thm] >>
     simp_tac bool_ss [BIT2, TWO, ONE, MULT_CLAUSES, ADD_CLAUSES]
   ]);
-
-val bit_induction = prove(
-  ``!P. P 0 /\ (!n. P n ==> P (2 * n + 1)) /\
-        (!n. P n ==> P (2 * n + 2)) ==>
-        !n. P n``,
-  gen_tac >> strip_tac >> completeInduct_on `n` >> simp[] >>
-  qspec_then `n` strip_assume_tac bit_cases >> simp[]);
 
 val lrlemma1 = prove(
   ``lrnext (i + lrnext i) = 2 * lrnext i``,
@@ -654,6 +644,27 @@ val lrlemma2 = prove(
   `2 * i + (4 * lrnext i + 2) = 2 * (i + 2 * lrnext i) + 2`
      by decide_tac >> simp[lrnext212])
 
+val spt_acc_eqn = Q.store_thm("spt_acc_eqn",
+  `∀k i. spt_acc i k = lrnext i * k + i`,
+  ho_match_mp_tac bit_induction
+  \\ rw[]
+  >- rw[spt_acc_def]
+  >- (
+    rw[Once spt_acc_thm]
+    >- fs[EVEN_ODD,lemmas]
+    \\ simp[MULT2_DIV']
+    \\ simp[lrlemma1] )
+  >- (
+    ONCE_REWRITE_TAC[spt_acc_thm]
+    \\ simp[]
+    \\ reverse(rw[])
+    >- fs[EVEN_ODD,lemmas]
+    \\ simp[MULT2_DIV']
+    \\ simp[lrlemma2]));
+
+val spt_acc_0 = Q.store_thm("spt_acc_0",
+  `∀k. spt_acc 0 k = k`, rw[spt_acc_eqn,lrnext_thm]);
+
 val set_foldi_keys = store_thm(
   "set_foldi_keys",
   ``!t a i. foldi (\k v a. k INSERT a) i a t =
@@ -672,6 +683,33 @@ val domain_foldi = save_thm(
                  |> SIMP_RULE (srw_ss()) [lrnext_thm]
                  |> SYM);
 val _ = computeLib.add_persistent_funs ["domain_foldi"]
+
+val mapi0_def = Define`
+  (mapi0 f i LN = LN) /\
+  (mapi0 f i (LS a) = LS (f i a)) /\
+  (mapi0 f i (BN t1 t2) =
+   let inc = lrnext i in
+     mk_BN (mapi0 f (i + 2 * inc) t1) (mapi0 f (i + inc) t2)) /\
+  (mapi0 f i (BS t1 a t2) =
+   let inc = lrnext i in
+     mk_BS (mapi0 f (i + 2 * inc) t1) (f i a) (mapi0 f (i + inc) t2))
+`;
+val _ = export_rewrites ["mapi0_def"]
+val mapi_def = Define`mapi f pt = mapi0 f 0 pt`;
+
+val lookup_mapi0 = Q.store_thm("lookup_mapi0",
+  `∀pt i k.
+   lookup k (mapi0 f i pt) =
+   case lookup k pt of NONE => NONE
+   | SOME v => SOME (f (spt_acc i k) v)`,
+  Induct \\ rw[mapi0_def,lookup_def,lookup_mk_BN,lookup_mk_BS] \\ fs[]
+  \\ TRY (simp[spt_acc_eqn] \\ NO_TAC)
+  \\ CASE_TAC \\ simp[Once spt_acc_thm,SimpRHS]);
+
+val lookup_mapi = Q.store_thm("lookup_mapi",
+  `lookup k (mapi f pt) = OPTION_MAP (f k) (lookup k pt)`,
+  rw[mapi_def,lookup_mapi0,spt_acc_0]
+  \\ CASE_TAC \\ fs[]);
 
 val toAList_def = Define `
   toAList = foldi (\k v a. (k,v)::a) 0 []`
@@ -788,15 +826,6 @@ val toAList_inc = prove(
     simp[MAP_EQ_f] >>
     simp[lrnext_thm,pairTheory.UNCURRY,pairTheory.FORALL_PROD] >>
     simp[lrlemma1,lrlemma2] ))
-
-val lemmas = prove(
-    ``(!x. EVEN (2 * x + 2)) /\
-      (!x. ODD (2 * x + 1))``,
-    conj_tac >- (
-      simp[EVEN_EXISTS] >> rw[] >>
-      qexists_tac`SUC x` >> simp[] ) >>
-    simp[ODD_EXISTS,ADD1] >>
-    metis_tac[] )
 
 val ALL_DISTINCT_MAP_FST_toAList = store_thm("ALL_DISTINCT_MAP_FST_toAList",
   ``!t. ALL_DISTINCT (MAP FST (toAList t))``,
@@ -1460,27 +1489,15 @@ val MAP_foldi = Q.store_thm(
              foldi (\k v a. (f (k,v)::a)) n (MAP f acc) pt`,
   Induct_on `pt` >> simp[foldi_def]);
 
-
-(*
 val mapi_Alist = Q.store_thm(
   "mapi_Alist",
   `mapi f pt =
     fromAList (MAP (\kv. (FST kv,f (FST kv) (SND kv))) (toAList pt))`,
   simp[spt_eq_thm, wf_mapi, wf_fromAList, lookup_fromAList] >>
-  simp[mapi_def, ALOOKUP_MAP_lemma] >>
-  `!n i j. lookup n (mapi0 f i pt) =
-           ALOOKUP (MAP (\kv. (FST kv, f (FST kv + i) (SND kv)))
-                        (foldi (\k v a. (k,v)::a) 0 [] pt)) n`
-     suffices_by simp[] >>
-  Induct_on `pt` >>
-  >- simp[lookup_def, toAList_def, foldi_def]
-  >- (simp[lookup_def, toAList_def, foldi_def] >> rpt strip_tac >>
-      COND_CASES_TAC >> simp[])
-  >- (simp[lookup_def, lookup_mk_BN, foldi_def] >>
+  srw_tac[boolSimps.ETA_ss][lookup_mapi, ALOOKUP_MAP_lemma, ALOOKUP_toAList]);
 
-  simp[mapi0_def, toAList_def, foldi_def, fromAList_def, Once insert_def,
-       mk_BN_def, ALOOKUP_MAP_lemma, lookup_def] >> rpt strip_tac >>
-  >- (
-*)
+val domain_mapi = Q.store_thm("domain_mapi",
+  `domain (mapi f pt) = domain pt`,
+  rw[pred_setTheory.EXTENSION,domain_lookup,lookup_mapi]);
 
 val _ = export_theory();
